Quicksort.v
@@ -6,18 +6,119 @@ Definition quicksort_impl_right_predicate {A} (rb : A -> A -> bool) x := fun y =
 
 Definition quicksort_impl {A} rb :=
   fix quicksort_impl (n : nat) (l : list A) :=
-    match n, l with
-    | 0, [] => []
-    | S n', x :: l' =>
-      quicksort_impl n' (filter (quicksort_impl_left_predicate rb x) l') ++
-        x ::
-        quicksort_impl n' (filter (quicksort_impl_right_predicate rb x) l')
-    | _, _ => []
+    match n with
+    | 0 =>
+      match l with
+      | [] => []
+      | _ :: _ => []
+      end
+    | S n' =>
+      match l with
+      | [] => []
+      | x :: l' =>
+        quicksort_impl n' (filter (quicksort_impl_left_predicate rb x) l') ++
+          x ::
+          quicksort_impl n' (filter (quicksort_impl_right_predicate rb x) l')
+      end
     end.
 
 Definition quicksort {A} (r : A -> A -> Prop) {total_order : TotalOrder r}
   {rb} {decidable_binary_relation : DecidableBinaryRelation r rb} :=
   fun l => quicksort_impl rb (length l) l.
+
+Lemma quicksort_impl_enough_fuel :
+  forall {A} rb n m (l : list A),
+  length l <= n ->
+  length l <= m ->
+  quicksort_impl rb n l = quicksort_impl rb m l.
+Proof.
+  intros ? ? ?. induction n; intros ? ? ? ?.
+  - destruct m.
+    + auto.
+    + destruct l; simpl in H; try lia. auto.
+  - destruct m.
+    + destruct l; simpl in H0; try lia. auto.
+    + simpl. destruct l.
+      * auto.
+      * f_equal.
+        -- specialize (length_filter_le (quicksort_impl_left_predicate rb a) l) as ?.
+           simpl in H, H0. apply IHn; lia.
+        -- f_equal. specialize (length_filter_le (quicksort_impl_right_predicate rb a) l) as ?.
+           simpl in H, H0. apply IHn; lia.
+Qed.
+
+Theorem quicksort_correct :
+  forall {A} (r : A -> A -> Prop) {total_order : TotalOrder r}
+    {rb} {decidable_binary_relation : DecidableBinaryRelation r rb},
+  is_sorter r (quicksort r).
+Proof.
+  unfold is_sorter, quicksort. intros ? ? ? ? ? ?.
+  remember (length l) as n. assert (length l <= n) by lia; clear Heqn.
+  generalize dependent l. induction n using nat_strong_induction; intros l ?.
+  destruct n.
+  - destruct l.
+    + simpl. split.
+      * apply permutation_nil.
+      * auto.
+    + simpl in H0. lia.
+  - destruct l.
+    + simpl. split.
+      * apply permutation_nil.
+      * auto.
+    + simpl. unfold quicksort_impl_left_predicate, quicksort_impl_right_predicate. simpl in H0.
+      specialize (length_filter_le (fun y => negb (rb a y)) l) as ?.
+      specialize (length_filter_le (fun y => rb a y) l) as ?.
+      destruct (
+        H
+        (length (filter (fun y => negb (rb a y)) l))
+        ltac:(lia)
+        (filter (fun y => negb (rb a y)) l)
+        ltac:(lia)
+      ) as (? & ?).
+      destruct (
+        H
+        (length (filter (fun y => rb a y) l))
+        ltac:(lia)
+        (filter (fun y => rb a y) l)
+        ltac:(lia)
+      ) as (? & ?).
+      rewrite <- (quicksort_impl_enough_fuel _ n) in H3, H4, H5, H6; try lia. clear H H0 H1 H2.
+      split.
+      * clear H4 H6. apply permutation_insert.
+        assert (predicate_xor (fun y => negb (rb a y)) (fun y => rb a y)). {
+          unfold predicate_xor. intros x. destruct (rb a x); intuition auto.
+        }
+        specialize (permutation_filter l (fun y => negb (rb a y)) (fun y => rb a y) H) as ?; clear H.
+        eapply permutation_app_trans.
+        -- apply H0.
+        -- apply permutation_sym. auto.
+        -- apply permutation_sym. auto.
+      * apply sorted_app.
+        -- auto.
+        -- simpl. split.
+           ++ eapply list_forall_permutation.
+              ** apply permutation_sym. apply H5.
+              ** rewrite list_forall_list_in. intros b ?.
+                 rewrite list_in_filter in H. destruct H as (? & ?).
+                 destruct (DecidableBinaryRelation_spec r a b); try discriminate.
+                 auto.
+           ++ auto.
+        -- simpl. eapply list_forall_permutation.
+           ++ apply permutation_sym. apply H3.
+           ++ rewrite list_forall_list_in. intros b ?.
+              rewrite list_in_filter in H. destruct H as (? & ?). split.
+              ** destruct (DecidableBinaryRelation_spec r a b); try discriminate.
+                 specialize (TotalOrder_totality r a b); intuition auto.
+              ** eapply list_forall_permutation.
+                 --- apply permutation_sym. apply H5.
+                 --- rewrite list_forall_list_in. intros c ?.
+                     rewrite list_in_filter in H1. destruct H1 as (? & ?).
+                     destruct (DecidableBinaryRelation_spec r a b); try discriminate.
+                     destruct (DecidableBinaryRelation_spec r a c); try discriminate.
+                     destruct (DecidableBinaryRelation_spec r b a).
+                     +++ apply (TotalOrder_transitivity r) with a; auto.
+                     +++ specialize (TotalOrder_totality r a b); intuition auto.
+Qed.
 
 Definition quicksort_impl_left_predicate_cost {A} rb {rb_Cost : Cost (Signature [_; _] _) rb} :=
   ltac2:(
@@ -38,15 +139,15 @@ Definition quicksort_impl_right_predicate_cost {A} rb {rb_Cost : Cost (Signature
   ).
 
 #[export] Instance quicksort_impl_left_predicate_Cost {A}
-  (rb : A -> A -> bool) {rb_Cost : Cost (Signature [_; _] _) rb} x :
-  Cost (Signature [_] _) (quicksort_impl_left_predicate rb x) := {
-  cost_fun := quicksort_impl_left_predicate_cost rb x;
+  (rb : A -> A -> bool) {rb_Cost : Cost (Signature [_; _] _) rb} :
+  Cost (Signature [_; _] _) (quicksort_impl_left_predicate rb) := {
+  cost_fun := quicksort_impl_left_predicate_cost rb;
 }.
 
 #[export] Instance quicksort_impl_right_predicate_Cost {A}
-  (rb : A -> A -> bool) {rb_Cost : Cost (Signature [_; _] _) rb} x :
-  Cost (Signature [_] _) (quicksort_impl_right_predicate rb x) := {
-  cost_fun := quicksort_impl_right_predicate_cost rb x;
+  (rb : A -> A -> bool) {rb_Cost : Cost (Signature [_; _] _) rb} :
+  Cost (Signature [_; _] _) (quicksort_impl_right_predicate rb) := {
+  cost_fun := quicksort_impl_right_predicate_cost rb;
 }.
 
 Definition quicksort_impl_cost {A} rb {rb_Cost : Cost (Signature [_; _] _) rb} :=
@@ -66,7 +167,7 @@ Definition quicksort_impl_cost {A} rb {rb_Cost : Cost (Signature [_; _] _) rb} :
           @filter_cost
           _
           (quicksort_impl_left_predicate rb x)
-          (@quicksort_impl_left_predicate_Cost _ _ rb_Cost _)
+          (Cost_cons _ _ _ _ (@quicksort_impl_left_predicate_Cost _ _ rb_Cost) _)
         )
       );
       (
@@ -75,7 +176,7 @@ Definition quicksort_impl_cost {A} rb {rb_Cost : Cost (Signature [_; _] _) rb} :
           @filter_cost
           _
           (quicksort_impl_right_predicate rb x)
-          (@quicksort_impl_right_predicate_Cost _ _ rb_Cost _)
+          (Cost_cons _ _ _ _ (@quicksort_impl_right_predicate_Cost _ _ rb_Cost) _)
         )
       );
       (('(@app A), 2), '(@app_cost A))
@@ -85,9 +186,162 @@ Definition quicksort_impl_cost {A} rb {rb_Cost : Cost (Signature [_; _] _) rb} :
     ['(@quicksort_impl A rb)]
   ).
 
-Section Example.
+Theorem quicksort_impl_left_predicate_cost_constant_on_cost_constant_rb :
+  forall {A} (rb : A -> A -> bool) {rb_Cost : Cost (Signature [_; _] _) rb},
+  binary_cost_constant rb_Cost ->
+  binary_cost_constant (quicksort_impl_left_predicate_Cost rb).
+Proof.
+  intros ? ? ? ?. destruct H as (c & H). exists (c + 4). intros (a, b). specialize (H (a, b)).
+  simpl. unfold quicksort_impl_left_predicate_cost. lia.
+Qed.
 
-Print quicksort_impl_cost.
+Theorem quicksort_impl_right_predicate_cost_constant_on_cost_constant_rb :
+  forall {A} (rb : A -> A -> bool) {rb_Cost : Cost (Signature [_; _] _) rb},
+  binary_cost_constant rb_Cost ->
+  binary_cost_constant (quicksort_impl_right_predicate_Cost rb).
+Proof.
+  intros ? ? ? ?. destruct H as (c & H). exists (c + 4). intros (a, b). specialize (H (a, b)).
+  simpl. unfold quicksort_impl_right_predicate_cost. lia.
+Qed.
+
+Lemma quicksort_cost_enough_fuel :
+  forall {A} (r : A -> A -> Prop) {total_order : TotalOrder r}
+    {rb} {decidable_binary_relation : DecidableBinaryRelation r rb}
+    {rb_Cost : Cost (Signature [_; _] _) rb}
+    n m l,
+  length l <= n ->
+  length l <= m ->
+  quicksort_impl_cost rb n l = quicksort_impl_cost rb m l.
+Proof.
+  intros ? ? ? ? ? ? ? ?. generalize dependent n. induction m; intros ? ? ? ?.
+  - destruct n.
+    + lia.
+    + destruct l.
+      * auto.
+      * simpl in H0. lia.
+  - destruct n.
+    + destruct l.
+      * simpl. lia.
+      * simpl in H. lia.
+    + destruct l.
+      * simpl. lia.
+      * simpl. simpl in H. simpl in H0.
+        specialize (length_filter_le (quicksort_impl_left_predicate rb a) l) as ?.
+        specialize (length_filter_le (quicksort_impl_right_predicate rb a) l) as ?.
+        rewrite (IHm n (filter (quicksort_impl_left_predicate rb a) l) ltac:(lia) ltac:(lia)).
+        rewrite (IHm n (filter (quicksort_impl_right_predicate rb a) l) ltac:(lia) ltac:(lia)).
+        clear IHm.
+        rewrite (quicksort_impl_enough_fuel _  n m); try lia.
+        rewrite (quicksort_impl_enough_fuel _  n m); try lia.
+Qed.
+
+Theorem quicksort_cost_quadratic_on_cost_constant_rb :
+  forall {A} (r : A -> A -> Prop) {total_order : TotalOrder r}
+    {rb} {decidable_binary_relation : DecidableBinaryRelation r rb}
+    {rb_Cost : Cost (Signature [_; _] _) rb},
+  binary_cost_constant rb_Cost ->
+  big_o
+    (fun l => quicksort_impl_cost rb (length l) l)
+    (fun (l : list A) => 1 + (length l) * (length l)).
+Proof.
+  intros ? ? ? ? ? ? ?.
+  specialize (@app_cost_linear A) as ?.
+  specialize (
+    filter_cost_linear_when_predicate_cost_constant_binary
+    (quicksort_impl_left_predicate rb)
+    (quicksort_impl_left_predicate_cost_constant_on_cost_constant_rb rb H)
+  ) as ?.
+  specialize (
+    filter_cost_linear_when_predicate_cost_constant_binary
+    (quicksort_impl_right_predicate rb)
+    (quicksort_impl_right_predicate_cost_constant_on_cost_constant_rb rb H)
+  ) as ?.
+  clear H. destruct H0 as (c1 & H0), H1 as (c2 & H1), H2 as (c3 & H2).
+  exists ((c1 + c2 + c3) * 2 + 18). intros l.
+  remember (length l) as n. assert (length l <= n) by lia; clear Heqn.
+  generalize dependent l. induction n using nat_strong_induction; intros l ?.
+  destruct n.
+  - simpl. destruct l; lia.
+  - destruct l.
+    + simpl. lia.
+    + simpl. destruct (list_empty_or_not_empty l).
+      * subst l. destruct n.
+        -- simpl. lia.
+        -- simpl. lia.
+      * simpl in H3. apply le_S_n in H3.
+        specialize (length_filter_le (quicksort_impl_left_predicate rb a) l) as ?.
+        specialize (length_filter_le (quicksort_impl_right_predicate rb a) l) as ?.
+        specialize (
+          H0
+          (
+            (quicksort_impl rb (length l) (filter (quicksort_impl_left_predicate rb a) l)),
+            (a :: quicksort_impl rb (length l) (filter (quicksort_impl_right_predicate rb a) l))
+          )
+        ).
+        simpl in H0. do 2 rewrite (quicksort_impl_enough_fuel _ (length l) n) in H0; try lia.
+        le_chain H0; clear H0.
+        specialize (H1 (a, l)). simpl in H1. le_chain H1; clear H1.
+        specialize (H2 (a, l)). simpl in H2. le_chain H2; clear H2.
+        specialize (quicksort_correct r (filter (quicksort_impl_left_predicate rb a) l)) as (? & _).
+        apply permutation_length in H0.
+        unfold quicksort in H0. rewrite <- (quicksort_impl_enough_fuel _ n) in H0; try lia.
+        specialize (quicksort_correct r (filter (quicksort_impl_right_predicate rb a) l)) as (? & _).
+        apply permutation_length in H1.
+        unfold quicksort in H1. rewrite <- (quicksort_impl_enough_fuel _ n) in H1; try lia.
+        rewrite <- H0; clear H0. rewrite <- H1; clear H1.
+        rewrite (
+          quicksort_cost_enough_fuel
+          _
+          n
+          (length (filter (quicksort_impl_left_predicate rb a) l))
+          (filter (quicksort_impl_left_predicate rb a) l)
+          ltac:(lia)
+          ltac:(lia)
+        ).
+        rewrite (
+          quicksort_cost_enough_fuel
+          _
+          n
+          (length (filter (quicksort_impl_right_predicate rb a) l))
+          (filter (quicksort_impl_right_predicate rb a) l)
+          ltac:(lia)
+          ltac:(lia)
+        ).
+        specialize (
+          H
+          (length (filter (quicksort_impl_left_predicate rb a) l))
+          ltac:(lia)
+          (filter (quicksort_impl_left_predicate rb a) l)
+          ltac:(lia)
+        ) as ?. le_chain H0; clear H0.
+        specialize (
+          H
+          (length (filter (quicksort_impl_right_predicate rb a) l))
+          ltac:(lia)
+          (filter (quicksort_impl_right_predicate rb a) l)
+          ltac:(lia)
+        ) as ?. le_chain H0; clear H0.
+        clear H.
+        assert (predicate_xor (quicksort_impl_left_predicate rb a) (quicksort_impl_right_predicate rb a)). {
+          unfold quicksort_impl_left_predicate, quicksort_impl_right_predicate.
+          unfold predicate_xor. intros x. destruct (rb a x); intuition auto.
+        }
+        specialize (permutation_filter l _ _ H) as ?; clear H.
+        apply permutation_length in H0. rewrite length_app in H0.
+        replace (fun x => quicksort_impl_right_predicate rb a x)
+          with (quicksort_impl_right_predicate rb a) in H0 by auto.
+        remember (length (filter (quicksort_impl_left_predicate rb a) l)) as m.
+        remember (length (filter (quicksort_impl_right_predicate rb a) l)) as k.
+        rewrite H0 in *. repeat (eapply le_trans_rev; [le_chain_l H3 |]).
+        assert (length l >= 1). {
+          destruct l.
+          - destruct n0. auto.
+          - simpl. lia.
+        }
+        rewrite H0 in H. clear n0 Heqm Heqk H0 H3 H4 H5. nia.
+Qed.
+
+Section Example.
 
 Compute quicksort Nat.le [4; 4; 6; 1; 0; 40; 3].
 
